Update examples.

test/Example.v
@@ -155,6 +155,8 @@ Module ExampleTermKit <: (TermKit ExampleTypeKit).
 
   Definition 𝑹𝑬𝑮 : Ty -> Set := fun _ => Empty_set.
 
+  Definition 𝑨𝑫𝑫𝑹 : Set := Empty_set.
+
 End ExampleTermKit.
 Module ExampleTerms := Terms ExampleTypeKit ExampleTermKit.
 Import ExampleTerms.
@@ -204,19 +206,34 @@ Module ExampleProgramKit <: (ProgramKit ExampleTypeKit ExampleTermKit).
     end in exact pi.
   Defined.
 
-Definition RegStore := Empty_set.
+Definition RegStore : Set := Empty_set.
+
 Definition read_register (γ : RegStore) {σ} (r : 𝑹𝑬𝑮 σ) : Lit σ :=
   match r with end.
+
 Definition write_register (γ : RegStore) {σ} (r : 𝑹𝑬𝑮 σ) (v : Lit σ) : RegStore :=
   match r with end.
+
 Definition read_write (γ : RegStore) σ (r : 𝑹𝑬𝑮 σ) (v : Lit σ) :
     read_register (write_register γ r v) r = v := match r with end.
+
 Definition write_read (γ : RegStore) σ (r : 𝑹𝑬𝑮 σ) :
     (write_register γ r (read_register γ r)) = γ := match r with end.
+
 Definition write_write (γ : RegStore) σ (r : 𝑹𝑬𝑮 σ) (v1 v2 : Lit σ) :
     write_register (write_register γ r v1) r v2 = write_register γ r v2 :=
   match r with end.
+
+Definition Memory : Set := Empty_set.
+
+Definition read_memory (μ : Memory) (addr : 𝑨𝑫𝑫𝑹) : Lit ty_int :=
+  match addr with end.
+
+Definition write_memory (μ : Memory) (addr : 𝑨𝑫𝑫𝑹) (v : Lit ty_int) : Memory :=
+  match addr with end.
+
 End ExampleProgramKit.
+
 Module ExamplePrograms :=
   Programs ExampleTypeKit ExampleTermKit ExampleProgramKit.
 Import ExamplePrograms.
